finished forward correctness

TeryGrad/Minimal/mwe.lean
@@ -1,14 +1,36 @@
-example (A B : Array Nat) : A = B := by
-    ext i h1 h2
+import Batteries.Logic
+
+inductive DiffTree (α : Type u) (β : Type v) : List Nat → Type (max u v)
+| mk
+    (outShape : List Nat)
+    (parents : Array (Σ shape, DiffTree α β shape))
+    : DiffTree α β outShape
 
 
-/- case h₁
-    A B : Array Nat
-    ⊢ A.size = B.size
-case h₂
-    A B : Array Nat
-    i✝ : Nat
-    hi₁✝ : i✝ < A.size
-    hi₂✝ : i✝ < B.size
-    ⊢ A[i✝] = B[i✝]
+inductive DiffTree.valid {α : Type u} {β : Type v} : ∀ (shape : List Nat), DiffTree α β shape → Prop
+| mk (outShape : List Nat) (parents : Array (Σ shape, DiffTree α β shape)) : (DiffTree.mk outShape parents).valid
+
+example (shapeX : List Nat)
+    (X : DiffTree α β shapeX)
+    (shapeP : List Nat)
+    (P : DiffTree α β shapeP)
+    (H1 : shapeX = shapeP)
+    (H2 : HEq P X)
+    (hv : P.valid) : X.valid := by
+  cases H1
+  cases H2
+  exact hv
+
+/-
+  α : Type u_1
+β : Type u_2
+shapeX : List Nat
+X : DiffTree α β shapeX
+shapeP : List Nat
+P : DiffTree α β shapeP
+H : shapeX = shapeP ∧ HEq P X
+hv : DiffTree.valid shapeP P
+temp : DiffTree α β shapeX := cast ⋯ P
+this : temp = X
+⊢ DiffTree.valid shapeX (cast ⋯ P)
 -/
